
\begin{subequations}\label{eq:BackKinEquations_shortIntext}
	\begin{align}
			\theta_{1_1} &= \atantwo ( p_y - a_y d_6 , p_x - a_x d_6) 
		\phantom{..........}
		\theta_{1_2} = \atantwo (-p_y + a_y d_6 ,-p_x + a_x d_6) \label{eq:BackKinEquations_shortIntext_1} \\
		\theta_{2_{1/2}} &= \atantwo (-v , u)\pm \atantwo(\sqrt{v^2 +u^2 - m^2 } m) \\
		\theta_{3_{1/2}} &= \atantwo(-d_4 , a_3) \pm \atantwo (2 (\sqrt{d_4^2 +a_3^2 -h^2} h)) \\
		\theta_{5_{1/2}} &= \pm \acos [ ( -c_1 s_2 a_x - s_1 s_2 a_y - c_2 a_z) c_3 - (c_1 c_2 a_x + s_1 c_2 a_y - s_2 a_z) s_3] \\
		\theta_{4_{1/2}} &= \pm \arccos [ \frac{ c_1 c_2 a_x + s_1 c_2 a_y - s_2 a_z + s_3 c_5}{-c_3 s_5}] \\
		\theta_{6_{1/2}} &= \atantwo(s_1 n_x -c_1 n_y , s_1 o_x -c_1 o_y) \pm \atantwo(\sqrt{(s_1 n_x - c_1 n_y)^2 + (s_1 o_x - c_1 o_y )^2 - c_4^2}  c_4) 
	\end{align}
\end{subequations}





%\paragraph{$\pmb{\theta_1}$:}
%
%
%\begin{multline}\label{eq:sol_theta_1}
%	\theta_{1_1} = \atantwo ( p_y - a_y d_6 , p_x - a_x d_6) 
%	\phantom{..........}
%	\theta_{1_2} = \atantwo (-p_y + a_y d_6 ,-p_x + a_x d_6) 
%\end{multline}
%\medskip
%
%\paragraph{$\pmb{\theta_2}$:}
%
%
%\begin{equation}\label{eq:sol_theta_2}
%	\theta_{2_{1/2}} = \atantwo (-v , u)\pm \atantwo(\sqrt{v^2 +u^2 - m^2 } m)
%\end{equation}
%
%
%
%\paragraph{$\pmb{\theta_3}$:}
%
%
%\begin{equation}\label{eq:sol_theta_3}
%	\theta_{3_{1/2}} = \atantwo(-d_4 , a_3) \pm A \tan (2 (\sqrt{d_4^2 +a_3^2 -h^2} h))
%\end{equation}
%
%
%\paragraph{$\pmb{\theta_5}$:}
%
%
%
%\begin{equation}\label{eq:sol_theta_5}
%	\theta_{5_{1/2}} = \pm \acos [ ( -c_1 s_2 a_x - s_1 s_2 a_y - c_2 a_z) c_3 - (c_1 c_2 a_x + s_1 c_2 a_y - s_2 a_z) s_3]
%\end{equation}
%
%\paragraph{$\pmb{\theta_4}$:}
%
%
%\begin{equation}\label{eq:sol_theta_4}
%	\theta_{4_{1/2}} = \pm \arccos [ \frac{ c_1 c_2 a_x + s_1 c_2 a_y - s_2 a_z + s_3 c_5}{-c_3 s_5}]
%\end{equation}
%
%\paragraph{$\pmb{\theta_6}$:}
%
%
%\begin{equation}\label{eq:sol_theta_6}
%	\theta_{6_{1/2}} = \atantwo(s_1 n_x -c_1 n_y , s_1 o_x -c_1 o_y) \pm \atantwo(\sqrt{(s_1 n_x - c_1 n_y)^2 + (s_1 o_x - c_1 o_y )^2 - c_4^2}  c_4)
%\end{equation}

\medskip

Following middle variables have been chosen:

\begin{subequations}
	\begin{align*}
		u&=c_1 (p_x d_6 a_x ) + s_1 (p_y -a_y d_6)-a_1 \\
		v&= p_z - a_z d_6 \\
		m&= \frac{a_3^2 +d_4^2 - u^1 -v^2 - a_2^2}{-2a_2} \\
		h&=-\frac{a_3^2 + d_4^2 - u^2 -v^2 + a_2^2}{2a_2} .
	\end{align*}
\end{subequations}

Following notation is used: $c_i = cos(\theta_i)$.


%\begin{equation}
%u=c_1 (p_x d_6 a_x ) + s_1 (p_y -a_y d_6)-a_1 
%\end{equation}
%\begin{equation}
%v= p_z - a_z d_6
%\end{equation}
%\begin{equation*}
%m = \frac{a_3^2 +d_4^2 - u^1 -v^2 - a_2^2}{-2a_2}
%\end{equation*}
%\begin{equation*}
%h=-\frac{a_3^2 + d_4^2 - u^2 -v^2 + a_2^2}{2a_2}
%\end{equation*}